verif/indices/btree_normalized_funspecs.v
@@ -10,6 +10,19 @@ Require Import btrees.btrees.
 Require Import btrees.btrees_sep.
 Require Import btrees.btrees_spec.
 
+Definition normalized_RL_PutRecord_funspec : funspec :=
+  WITH r:relation val, c:cursor val, pc:val, key:key, recordptr:val, record:V, gv: globals
+  PRE[ 1%positive OF tptr tcursor, 2%positive OF size_t, 3%positive OF tptr tvoid ] 
+    PROP(complete_cursor c r; Z.succ (get_depth r) < MaxTreeDepth;
+             root_integrity (get_root r); root_wf (get_root r);
+             get_numrec r < Int.max_signed - 1)
+    LOCAL(gvars gv; temp 1%positive pc; temp 2%positive (Vptrofs key); temp 3%positive recordptr)
+    SEP(mem_mgr gv; relation_rep r (get_numrec r); cursor_rep c r pc; value_rep record recordptr)
+  POST[ tvoid ]
+    EX newc: cursor val,  EX newr: relation val,
+    PROP(RL_PutRecord_rel c r key record recordptr newr newc)
+    LOCAL()
+    SEP(mem_mgr gv * relation_rep newr (get_numrec newr) * cursor_rep newc newr pc).
 
 Definition normalized_goToKey_funspec : funspec :=
   WITH c:cursor val, pc:val, r:relation val, key:key, numrec:Z
@@ -22,23 +35,6 @@ Definition normalized_goToKey_funspec : funspec :=
     PROP()
     LOCAL()
     SEP(relation_rep r numrec; cursor_rep (goToKey c r key) r pc).
-
-
-Definition normalized_putRecord_funspec :=
-  WITH r:relation val, c:cursor val, pc:val, key:key, recordptr:val, record:V, gv: globals
-  PRE[ 1%positive OF tptr tcursor, 2%positive OF size_t, 3%positive OF tptr tvoid ] 
-    PROP(complete_cursor c r; Z.succ (get_depth r) < MaxTreeDepth;
-             root_integrity (get_root r); root_wf (get_root r);
-             get_numrec r < Int.max_signed - 1)
-    LOCAL(gvars gv; temp 1%positive pc; temp 2%positive (Vptrofs key); temp 3%positive recordptr)
-    SEP(mem_mgr gv; relation_rep r (get_numrec r); cursor_rep c r pc; value_rep record recordptr)
-  POST[ tvoid ]
-    EX newx:list val,
-    PROP()
-    LOCAL()
-    SEP(let (newc,newr) := RL_PutRecord c r key record recordptr newx nullval in
-        (mem_mgr gv * relation_rep newr (get_numrec newr) * cursor_rep newc newr pc)).
-
 
 Definition normalized_getRecord_funspec :=
   WITH r:relation val, c:cursor val, pc:val, numrec:Z
