verif/indices/ordered_interface.v
@@ -2,13 +2,6 @@ Require Import VST.floyd.functional_base VST.floyd.proofauto.
 Require Import Coq.ZArith.BinInt.
 Require Import indices.unordered_flat.
 Require Import VST.floyd.library.
-
-Infix ">=" := Z.geb : Z_scope.
-Infix "<=" := Z.leb : Z_scope.
-Infix "<" := Z.ltb: Z_scope.
-Infix ">" := Z.gtb: Z_scope.
-Infix "=" := Z.eqb: Z_scope.
-
 Module OrderedIndex.
 
 Record index :=
@@ -21,9 +14,10 @@ Record index :=
     
     value : Type;
     default_value: Inhabitant value;
+    value_repr: value -> val -> mpred;
 
     t: Type;
-    t_repr: t -> Z -> mpred;
+    t_repr: t -> Z -> val -> mpred;
     t_type: type;
     
     cursor : Type;
@@ -33,16 +27,15 @@ Record index :=
     (* helpers *)
     valid_cursor: cursor -> bool;
     norm: cursor -> cursor;
-    get_num_rec_levels: t -> Z;
+    rec_levels: cursor -> Z;
 
     (* interface *)
 
     create_cursor: t -> cursor;
-    create: val -> val -> t;
+    create_index: t -> Prop;
     
     cardinality: cursor -> Z;
 
-    (* this is like get_cursor in unordered *)
     go_to_key: cursor -> key -> cursor;
 
     move_to_next: cursor -> cursor;
@@ -55,9 +48,11 @@ Record index :=
    
     get_record: cursor -> val;
 
-    put_record: cursor -> key -> value -> val -> list val -> cursor;
+    put_record: cursor -> key -> value -> val -> cursor -> Prop;
 
   }.
+
+
 
 (* ================= VERIFIED =============== *)
 
@@ -73,48 +68,18 @@ Definition go_to_key_spec
     LOCAL()
     SEP(oi.(cursor_repr) (oi.(go_to_key) cur key) pc numrec).
 
-Definition create_spec (oi: OrderedIndex.index): funspec :=
-  (* what is unit for? *)
+Definition create_index_spec (oi: OrderedIndex.index): funspec :=
   WITH u:unit, gv: globals
   PRE [ ]
     PROP ()
     LOCAL (gvars gv)
     SEP (mem_mgr gv)
   POST [ tptr oi.(t_type) ]
-    EX pr:val, EX pn:val, 
-    PROP ()
+    EX m: oi.(t), EX pr: val,
+    PROP (oi.(create_index) m)
     LOCAL(temp ret_temp pr)
-    SEP (mem_mgr gv; oi.(t_repr) (oi.(create) pr pn) 0).
+    SEP (mem_mgr gv; oi.(t_repr) m 0 pr). 
 
-(* 
-Definition put_record_spec
-  (oi: OrderedIndex.index): funspec :=
-  WITH cur: oi.(cursor), m: oi.(t), pc:val, key:oi.(key), recordptr:val, record:oi.(value), gv: globals
-  PRE[ 1%positive OF tptr oi.(cursor_type), 2%positive OF oi.(key_type), 3%positive OF tptr tvoid ] 
-    PROP()
-    LOCAL(gvars gv; temp 1%positive pc; temp 2%positive (oi.(key_val) key); temp 3%positive recordptr)
-    SEP(mem_mgr gv; oi.(cursor_repr) cur pc (oi.(get_num_rec_levels) m))
-  POST[ tvoid ]
-    EX newx:list val,
-    PROP()
-    LOCAL()
-    SEP(let newc := oi.(put_record) cur key record recordptr newx in 
-        (mem_mgr gv * oi.(cursor_repr) newc pc (oi.(get_num_rec_levels) newr) )). *)
-
-(*Definition normalized_putRecord_funspec :=
-  WITH r:relation val, c:cursor val, pc:val, key:key, recordptr:val, record:V, gv: globals
-  PRE[ 1%positive OF tptr tcursor, 2%positive OF size_t, 3%positive OF tptr tvoid ] 
-    PROP(complete_cursor c r; Z.succ (get_depth r) < MaxTreeDepth;
-             root_integrity (get_root r); root_wf (get_root r);
-             get_numrec r < Int.max_signed - 1)
-    LOCAL(gvars gv; temp 1%positive pc; temp 2%positive (key_repr key); temp 3%positive recordptr)
-    SEP(mem_mgr gv; relation_rep r (get_numrec r); cursor_rep c r pc; value_rep record recordptr)
-  POST[ tvoid ]
-    EX newx:list val,
-    PROP()
-    LOCAL()
-    SEP(let (newc,newr) := RL_PutRecord c r key record recordptr newx nullval in
-        (mem_mgr gv * relation_rep newr (get_numrec newr) * cursor_rep newc newr pc)). *)
 
 Definition create_cursor_spec
   (oi: OrderedIndex.index): funspec :=
@@ -122,7 +87,7 @@ Definition create_cursor_spec
   PRE [ 1%positive OF tptr oi.(t_type)]
     PROP()
     LOCAL(gvars gv; temp 1%positive p)
-    SEP(mem_mgr gv; oi.(t_repr) r numrec)
+    SEP(mem_mgr gv; oi.(t_repr) r numrec p)
   POST [tptr oi.(cursor_type)]
     EX p':val,
     PROP()
@@ -200,5 +165,18 @@ Definition get_record_spec
     PROP()
     LOCAL(temp ret_temp (oi.(get_record) cur))
     SEP(oi.(cursor_repr) (oi.(norm) cur) p numrec).
+
+Definition put_record_spec 
+  (oi: OrderedIndex.index): funspec :=
+   WITH cur: oi.(cursor), pc:val, key:oi.(key), recordptr:val, record:oi.(value), gv: globals
+  PRE [ 1%positive OF tptr oi.(cursor_type), 2%positive OF oi.(key_type), 3%positive OF tptr tvoid]
+    PROP()
+    LOCAL(gvars gv; temp 1%positive pc; temp 2%positive (oi.(key_val) key); temp 3%positive recordptr)
+    SEP(mem_mgr gv; oi.(cursor_repr) cur pc (oi.(rec_levels) cur) * oi.(value_repr) record recordptr)
+  POST [tvoid]
+    EX newc: oi.(cursor), 
+    PROP(oi.(put_record) cur key record recordptr newc)
+    LOCAL()
+    SEP(mem_mgr gv; oi.(cursor_repr) newc pc (oi.(rec_levels) newc)).
 
 End OrderedIndex.
